thys/JinjaThreads/Examples/ApprenticeChallenge.thy
@@ -1,0 +1,107 @@
+(*  Title:      JinjaThreads/Examples/AppenticeChallenge.thy
+    Author:     Andreas Lochbihler
+*)
+
+header {* \chapter{Examples}
+          \isaheader{Apprentice challenge} *}
+theory ApprenticeChallenge 
+imports
+  "../Execute/Code_Generation"
+begin
+
+text {* This theory implements the apprentice challenge by Porter and Moore \cite{MoorePorter2002TOPLAS}. *}
+
+definition ThreadC :: "addr J_mb cdecl"
+where 
+  "ThreadC = 
+  (Thread, Object, [], 
+    [(run, [], Void, \<lfloor>([], unit)\<rfloor>),
+     (start, [], Void, Native),
+     (join, [], Void, Native),
+     (interrupt, [], Void, Native),
+     (isInterrupted, [], Boolean, Native)])"
+
+definition Container :: cname
+where "Container = STR ''Container''"
+
+definition ContainerC :: "addr J_mb cdecl"
+where "ContainerC = (Container, Object, [(STR ''counter'', Integer, \<lparr>volatile=False\<rparr>)], [])"
+
+definition String :: cname
+where "String = STR ''String''"
+
+definition StringC :: "addr J_mb cdecl"
+where
+  "StringC = (String, Object, [], [])"
+
+definition Job :: cname
+where "Job = STR ''Job''"
+
+definition JobC :: "addr J_mb cdecl"
+where
+  "JobC =
+  (Job, Thread, [(STR ''objref'', Class Container, \<lparr>volatile=False\<rparr>)],
+   [(STR ''incr'', [], Class Job, \<lfloor>([],
+     sync(Var (STR ''objref''))
+         ((Var (STR ''objref''))\<bullet>STR ''counter''{STR []} := ((Var (STR ''objref''))\<bullet>STR ''counter''{STR []} \<guillemotleft>Add\<guillemotright> Val (Intg 1)));;
+     Var this)\<rfloor>),
+    (STR ''setref'', [Class Container], Void, \<lfloor>([STR ''o''],
+     LAss (STR ''objref'') (Var (STR ''o'')))\<rfloor>),
+    (run, [], Void, \<lfloor>([],
+     while (true) (Var this\<bullet>STR ''incr''([])))\<rfloor>)
+    ])"
+
+definition Apprentice :: cname
+where "Apprentice = STR ''Apprentice''"
+
+definition ApprenticeC :: "addr J_mb cdecl"
+where
+  "ApprenticeC =
+  (Apprentice, Object, [],
+   [(STR ''main'', [Class String\<lfloor>\<rceil>], Void, \<lfloor>([STR ''args''],
+    {STR ''container'':Class Container=None;
+       (STR ''container'' := new Container);;
+       (while (true) 
+          {STR ''job'':Class Job=None;
+              (STR ''job'' := new Job);;
+              (Var (STR ''job'')\<bullet>STR ''setref''([Var (STR ''container'')]));;
+              (Var (STR ''job'')\<bullet>Type.start([]))
+          }
+       )
+    })\<rfloor>)])"
+
+definition ApprenticeChallenge
+where
+  "ApprenticeChallenge = Program (SystemClasses @ [StringC, ThreadC, ContainerC, JobC, ApprenticeC])"
+
+definition ApprenticeChallenge_annotated
+where "ApprenticeChallenge_annotated = annotate_prog_code ApprenticeChallenge"
+
+lemma "wf_J_prog ApprenticeChallenge_annotated"
+by eval
+
+lemmas [code_unfold] = 
+  Container_def Job_def String_def Apprentice_def
+
+definition main :: "String.literal" where "main = STR ''main''"
+
+ML {*
+  val program = @{code ApprenticeChallenge_annotated};
+  val compiled = @{code J2JVM} program;
+
+  @{code exec_J_rr}
+    @{code "1 :: nat"}
+    program
+    @{code Apprentice}
+    @{code main}
+    [ @{code Null}];
+
+  @{code exec_JVM_rr} 
+    @{code "1 :: nat"}
+    compiled
+    @{code Apprentice}
+    @{code main}
+    [ @{code Null}];
+*}
+
+end
