thys/JinjaThreads/Execute/Execute_Main.thy
@@ -2,9 +2,9 @@ theory Execute_Main
 imports
   SC_Schedulers
   PCompilerRefine
-  J_Execute
+  Code_Generation
   JVM_Execute
-  JVM_Execute2
+  Java2Jinja
 begin
 
 end
