thys/JinjaThreads/Execute/Java2Jinja.thy
@@ -1,0 +1,77 @@
+(*  Title:      JinjaThreads/Execute/Java2Jinja.thy
+    Author:     Andreas Lochbihler
+*)
+
+header {* \isaheader{Setup for converter Java2Jinja} *}
+theory Java2Jinja 
+imports
+  Code_Generation
+  ToString
+begin
+
+code_modulename SML
+  Java2Jinja Code_Generation
+
+definition j_Program :: "addr J_mb cdecl list \<Rightarrow> addr J_prog"
+where "j_Program = Program"
+
+export_code wf_J_prog' j_Program in SML file "JWellForm.ML" 
+
+text {* Functions for extracting calls to the native print method *}
+
+definition purge where
+  "\<And>run.
+  purge run = 
+  lmap (\<lambda>obs. case obs of ExternalCall _ _ (Cons (Intg i) _) v \<Rightarrow> i)
+  (lfilter
+    (\<lambda>obs. case obs of ExternalCall _ M (Cons (Intg i) Nil) _ \<Rightarrow> M = print | _ \<Rightarrow> False) 
+    (lconcat (lmap (llist_of \<circ> snd) (llist_of_tllist run))))"
+
+text {* Various other functions *}
+
+instantiation heapobj :: toString begin
+primrec toString_heapobj :: "heapobj \<Rightarrow> String.literal" where
+  "toString (Obj C fs) = Aux.concat [STR ''(Obj '', toString C, STR '', '', toString fs, STR '')'']"
+| "toString (Arr T si fs el) = 
+   Aux.concat [STR ''(['', toString si, STR '']'', toString T, STR '', '', toString fs, STR '', '', toString (map snd (rm_to_list el)), STR '')'']"
+instance proof qed
+end
+
+definition llist_case' where "llist_case' = llist_case"
+definition tllist_case' where "tllist_case' = tllist_case"
+definition terminal' where "terminal' = terminal"
+definition llist_of_tllist' where "llist_of_tllist' = llist_of_tllist"
+definition thr' where "thr' = thr"
+definition shr' where "shr' = shr"
+
+definition heap_toString :: "heap \<Rightarrow> String.literal"
+where "heap_toString = toString"
+
+definition thread_toString :: "(thread_id, (addr expr \<times> addr locals) \<times> (addr \<Rightarrow>\<^isub>f nat)) rbt \<Rightarrow> String.literal"
+where "thread_toString = toString"
+
+definition thread_toString' :: "(thread_id, addr jvm_thread_state' \<times> (addr \<Rightarrow>\<^isub>f nat)) rbt \<Rightarrow> String.literal"
+where "thread_toString' = toString"
+
+definition trace_toString :: "thread_id \<times> (addr, thread_id) obs_event list \<Rightarrow> String.literal"
+where "trace_toString = toString"
+
+export_code
+  wf_J_prog' exec_J_rr exec_J_rnd 
+  j_Program
+  purge llist_case' tllist_case' terminal' llist_of_tllist'
+  thr' shr' heap_toString thread_toString trace_toString
+  in SML
+  file "J_Execute.ML"
+
+definition j2jvm :: "addr J_prog \<Rightarrow> addr jvm_prog" where "j2jvm = J2JVM"
+
+export_code
+  wf_jvm_prog' exec_JVM_rr exec_JVM_rnd j2jvm
+  j_Program 
+  purge llist_case' tllist_case' terminal' llist_of_tllist'
+  thr' shr' heap_toString thread_toString' trace_toString
+  in SML
+  file "JVM_Execute2.ML"
+
+end
