thys/JinjaThreads/Execute/ToString.thy
@@ -1,0 +1,288 @@
+(*  Title:      JinjaThreads/Execute/ToString.thy
+    Author:     Andreas Lochbihler
+*)
+
+header {* \isaheader{String representation of types} *}
+theory ToString imports 
+  "../J/Expr"
+  "../JVM/JVMInstructions"
+  "../../Collections/TrieMapImpl"
+  "../../Collections/RBTMapImpl"
+  "../../Collections/Assoc_List"
+begin
+
+class toString =
+  fixes toString :: "'a \<Rightarrow> String.literal"
+
+instantiation bool :: toString begin
+definition [code]: "toString b = (case b of True \<Rightarrow> STR ''True'' | False \<Rightarrow> STR ''False'')"
+instance proof qed
+end
+
+instantiation char :: toString begin
+definition [code]: "toString (c :: char) = implode [c]"
+instance proof qed
+end
+
+instantiation String.literal :: toString begin
+definition [code]: "toString (s :: String.literal) = s"
+instance proof qed
+end
+
+fun list_toString :: "String.literal \<Rightarrow> 'a :: toString list \<Rightarrow> String.literal list"
+where
+  "list_toString sep [] = []"
+| "list_toString sep [x] = [toString x]"
+| "list_toString sep (x#xs) = toString x # sep # list_toString sep xs"
+
+instantiation list :: (toString) toString begin
+definition [code]:
+  "toString (xs :: 'a list) = Aux.concat (STR ''['' # list_toString (STR '','') xs @ [STR '']''])"
+instance proof qed
+end
+
+function digit_toString :: "int \<Rightarrow> String.literal"
+where
+  "digit_toString 0 = STR ''0''"
+| "digit_toString 1 = STR ''1''"
+| "digit_toString 2 = STR ''2''"
+| "digit_toString 3 = STR ''3''"
+| "digit_toString 4 = STR ''4''"
+| "digit_toString 5 = STR ''5''"
+| "digit_toString 6 = STR ''6''"
+| "digit_toString 7 = STR ''7''"
+| "digit_toString 8 = STR ''8''"
+| "digit_toString 9 = STR ''9''"
+| "n \<notin> {0, 1, 2, 3, 4, 5, 6, 7, 8, 9} \<Longrightarrow> digit_toString n = undefined"
+apply(case_tac x)
+apply simp_all
+apply(rename_tac n', case_tac n', simp)
+apply(rename_tac n', case_tac n', simp)
+apply(rename_tac n', case_tac n', simp)
+apply(rename_tac n', case_tac n', simp)
+apply(rename_tac n', case_tac n', simp)
+apply(rename_tac n', case_tac n', simp)
+apply(rename_tac n', case_tac n', simp)
+apply(rename_tac n', case_tac n', simp)
+apply(rename_tac n', case_tac n', simp)
+apply(rename_tac n', case_tac n', simp)
+apply simp
+done
+termination by lexicographic_order
+
+function int_toString :: "int \<Rightarrow> String.literal list"
+where
+  "int_toString n = 
+  (if n < 0 then STR ''-'' # int_toString (- n)
+   else if n < 10 then [digit_toString n ]
+   else int_toString (n div 10) @ [digit_toString (n mod 10)])"
+by pat_completeness simp
+termination by size_change
+
+instantiation int :: toString begin
+definition [code]: "toString i = Aux.concat (int_toString i)"
+instance proof qed
+end
+
+instantiation nat :: toString begin
+definition [code]: "toString n = toString (int n)"
+instance proof qed
+end
+
+instantiation option :: (toString) toString begin
+primrec toString_option :: "'a option \<Rightarrow> String.literal" where
+  "toString None = STR ''None''"
+| "toString (Some a) = Aux.concat [STR ''Some ('', toString a, STR '')'']"
+instance proof qed
+end
+
+instantiation finfun :: ("{toString, card_UNIV, equal, linorder}", toString) toString begin
+definition [code]: 
+  "toString (f :: 'a \<Rightarrow>\<^isub>f 'b) = 
+   Aux.concat 
+     (STR ''('' 
+     # toString (finfun_default f) 
+     # concat (map (\<lambda>x. [STR '','', toString x, STR ''|->'', toString (f\<^sub>f x)]) (finfun_to_list f)) 
+     @ [STR '')''])"
+instance proof qed
+end
+
+instantiation word :: (len) toString begin
+definition [code]: "toString (w :: 'a word) = toString (sint w)"
+instance proof qed
+end
+
+instantiation "fun" :: (type, type) toString begin
+definition [code]: "toString (f :: 'a \<Rightarrow> 'b) = STR ''fn''"
+instance proof qed
+end
+
+instantiation val :: (toString) toString begin
+fun toString_val :: "('a :: toString) val \<Rightarrow> String.literal"
+where
+  "toString Unit = STR ''Unit''"
+| "toString Null = STR ''Null''"
+| "toString (Bool b) = Aux.concat [STR ''Bool '', toString b]"
+| "toString (Intg i) = Aux.concat [STR ''Intg '', toString i]"
+| "toString (Addr a) = Aux.concat [STR ''Addr '', toString a]"
+instance proof qed
+end
+
+instantiation ty :: toString begin
+primrec toString_ty :: "ty \<Rightarrow> String.literal"
+where
+  "toString Void = STR ''Void''"
+| "toString Boolean = STR ''Boolean''"
+| "toString Integer = STR ''Integer''"
+| "toString NT = STR ''NT''"
+| "toString (Class C) = Aux.concat [STR ''Class '', toString C]"
+| "toString (T\<lfloor>\<rceil>) = Aux.concat [toString T, STR ''[]'']"
+instance proof qed
+end
+
+instantiation bop :: toString begin
+primrec toString_bop :: "bop \<Rightarrow> String.literal" where
+  "toString Eq = STR ''==''"
+| "toString NotEq = STR ''!=''"
+| "toString LessThan = STR ''<''"
+| "toString LessOrEqual = STR ''<=''"
+| "toString GreaterThan = STR ''>''"
+| "toString GreaterOrEqual = STR ''>=''"
+| "toString Add = STR ''+''"
+| "toString Subtract = STR ''-''"
+| "toString Mult = STR ''*''"
+| "toString Div = STR ''/''"
+| "toString Mod = STR ''%''"
+| "toString BinAnd = STR ''&''"
+| "toString BinOr = STR ''|''"
+| "toString BinXor = STR ''^''"
+| "toString ShiftLeft = STR ''<<''"
+| "toString ShiftRightZeros = STR ''>>''"
+| "toString ShiftRightSigned = STR ''>>>''"
+instance proof qed
+end
+
+instantiation addr_loc :: toString begin
+primrec toString_addr_loc :: "addr_loc \<Rightarrow> String.literal" where
+  "toString (CField C F) = Aux.concat [STR ''CField '', F, STR ''{'', C, STR ''}'']"
+| "toString (ACell n) = Aux.concat [STR ''ACell '', toString n]"
+instance proof qed
+end
+
+instantiation htype :: toString begin
+fun toString_htype :: "htype \<Rightarrow> String.literal" where
+  "toString (Class_type C) = C"
+| "toString (Array_type T n) = Aux.concat [toString T, STR ''['', toString n, STR '']'']"
+instance proof qed
+end
+
+instantiation obs_event :: (toString, toString) toString begin
+primrec toString_obs_event :: "('a :: toString, 'b :: toString) obs_event \<Rightarrow> String.literal"
+where
+  "toString (ExternalCall ad M vs v) = 
+   Aux.concat [STR ''ExternalCall '', M, STR ''('', toString vs, STR '') = '', toString v]"
+| "toString (ReadMem ad al v) =
+   Aux.concat [STR ''ReadMem '', toString ad, STR ''@'', toString al, STR ''='', toString v]"
+| "toString (WriteMem ad al v) =
+   Aux.concat [STR ''WriteMem '', toString ad, STR ''@'', toString al, STR ''='', toString v]"
+| "toString (NewHeapElem ad hT) = Aux.concat [STR ''Allocate '', toString ad, STR '':'', toString hT]"
+| "toString (ThreadStart t) = Aux.concat [STR ''ThreadStart '', toString t]"
+| "toString (ThreadJoin t) = Aux.concat [STR ''ThreadJoin '', toString t]"
+| "toString (SyncLock ad) = Aux.concat [STR ''SyncLock '', toString ad]"
+| "toString (SyncUnlock ad) = Aux.concat [STR ''SyncUnlock '', toString ad]"
+| "toString (ObsInterrupt t) = Aux.concat [STR ''Interrupt '', toString t]"
+| "toString (ObsInterrupted t) = Aux.concat [STR ''Interrupted '', toString t]"
+instance proof qed
+end
+
+instantiation prod :: (toString, toString) toString begin
+definition "toString = (\<lambda>(a, b). Aux.concat [STR ''('', toString a, STR '', '', toString b, STR '')''])"
+instance proof qed
+end
+
+instantiation fmod_ext :: (toString) toString begin
+definition "toString fd = Aux.concat [STR ''{|volatile='', toString (volatile fd), STR '', '', toString (fmod.more fd), STR ''|}'']"
+instance proof qed
+end
+
+instantiation unit :: toString begin
+definition "toString (u :: unit) = STR ''()''"
+instance proof qed
+end
+
+instantiation exp :: (toString, toString, toString) toString begin
+fun toString_exp :: "('a :: toString, 'b :: toString, 'c :: toString) exp \<Rightarrow> String.literal"
+where
+  "toString (new C) = Aux.concat [STR ''new '', C]"
+| "toString (newArray T e) = Aux.concat [STR ''new '', toString T, STR ''['', toString e, STR '']'']"
+| "toString (Cast T e) = Aux.concat [STR ''('', toString T, STR '') ('', toString e, STR '')'']"
+| "toString (InstanceOf e T) = Aux.concat [STR ''('', toString e, STR '') instanceof '', toString T]"
+| "toString (Val v) = Aux.concat [STR ''Val ('', toString v, STR '')'']"
+| "toString (e1 \<guillemotleft>bop\<guillemotright> e2) = Aux.concat [STR ''('', toString e1, STR '') '', toString bop, STR '' ('', toString e2, STR '')'']"
+| "toString (Var V) = Aux.concat [STR ''Var '', toString V]"
+| "toString (V := e) = Aux.concat [toString V, STR '' := ('', toString e, STR '')'']"
+| "toString (AAcc a i) = Aux.concat [STR ''('', toString a, STR '')['', toString i, STR '']'']"
+| "toString (AAss a i e) = Aux.concat [STR ''('', toString a, STR '')['', toString i, STR ''] := ('', toString e, STR '')'']"
+| "toString (ALen a) = Aux.concat [STR ''('', toString a, STR '').length'']"
+| "toString (FAcc e F D) = Aux.concat [STR ''('', toString e, STR '').'', F, STR ''{'', D, STR ''}'']"
+| "toString (FAss e F D e') = Aux.concat [STR ''('', toString e, STR '').'', F, STR ''{'', D, STR ''} := ('', toString e', STR '')'']"
+| "toString (Call e M es) = Aux.concat ([STR ''('', toString e, STR '').'', M, STR ''(''] @ map toString es @ [STR '')''])"
+| "toString (Block V T vo e) = Aux.concat ([STR ''{'', toString V, STR '':'', toString T] @ (case vo of None \<Rightarrow> [] | Some v \<Rightarrow> [STR ''='', toString v]) @ [STR ''; '', toString e, STR ''}''])"
+| "toString (Synchronized V e e') = Aux.concat [STR ''synchronized_'', toString V, STR ''_('', toString e, STR '') {'', toString e', STR ''}'']"
+| "toString (InSynchronized V ad e) = Aux.concat [STR ''insynchronized_'', toString V, STR ''_('', toString ad, STR '') {'', toString e, STR ''}'']"
+| "toString (e;;e') = Aux.concat [toString e, STR ''; '', toString e']"
+| "toString (if (e) e' else e'') = Aux.concat [STR ''if ('', toString e, STR '') { '', toString e', STR '' } else { '', toString e'', STR ''}'']"
+| "toString (while (e) e') = Aux.concat [STR ''while ('', toString e, STR '') { '', toString e', STR '' }'']"
+| "toString (throw e) = Aux.concat [STR ''throw ('', toString e, STR '')'']"
+| "toString (try e catch(C V) e') = Aux.concat [STR ''try { '', toString e, STR '' } catch ('', C, STR '' '', toString V, STR '') { '', toString e', STR '' }'']"
+instance proof qed
+end
+
+instantiation instr :: (toString) toString begin
+primrec toString_instr :: "'a instr \<Rightarrow> String.literal" where
+  "toString (Load i) = Aux.concat [STR ''Load ('', toString i, STR '')'']"
+| "toString (Store i) = Aux.concat [STR ''Store ('', toString i, STR '')'']"
+| "toString (Push v) = Aux.concat [STR ''Push ('', toString v, STR '')'']"
+| "toString (New C) = Aux.concat [STR ''New '', toString C]"
+| "toString (NewArray T) = Aux.concat [STR ''NewArray '', toString T]"
+| "toString ALoad = STR ''ALoad''"
+| "toString AStore = STR ''AStore''"
+| "toString ALength = STR ''ALength''"
+| "toString (Getfield F D) = Aux.concat [STR ''Getfield  '', toString F, STR '' '', toString D]"
+| "toString (Putfield F D) = Aux.concat [STR ''Putfield  '', toString F, STR '' '', toString D]"
+| "toString (Checkcast T) = Aux.concat [STR ''Checkcast '', toString T]"
+| "toString (Instanceof T) = Aux.concat [STR ''Instanceof '', toString T]"
+| "toString (Invoke M n) =  Aux.concat [STR ''Invoke '', toString M, STR '' '', toString n]"
+| "toString Return = STR ''Return''"
+| "toString Pop = STR ''Pop''"
+| "toString Dup = STR ''Dup''"
+| "toString Swap = STR ''Swap''"
+| "toString (BinOpInstr bop) = Aux.concat [STR ''BinOpInstr  '', toString bop]"
+| "toString (Goto i) = Aux.concat [STR ''Goto '', toString i]"
+| "toString (IfFalse i) = Aux.concat [STR ''IfFalse '', toString i]"
+| "toString ThrowExc = STR ''ThrowExc''"
+| "toString MEnter = STR ''monitorenter''"
+| "toString MExit = STR ''monitorexit''"
+instance proof qed
+end
+
+instantiation trie :: (toString, toString) toString begin
+definition [code]: "toString (t :: ('a, 'b) trie) = toString (tm_to_list t)"
+instance proof qed
+end
+
+instantiation rbt :: ("{toString,linorder}", toString) toString begin
+definition [code]: 
+  "toString (t :: ('a, 'b) rbt) = 
+   Aux.concat (list_toString (STR [Char Nibble2 NibbleC, Char Nibble0 NibbleA]) (rm_to_list t))"
+instance proof qed
+end
+
+instantiation assoc_list :: (toString, toString) toString begin
+definition [code]: "toString = toString \<circ> Assoc_List.impl_of"
+instance proof qed
+end
+
+code_instance String.literal :: toString (Haskell -)
+
+end
