thys/JinjaThreads/MM/JMM_J.thy
@@ -1,0 +1,35 @@
+theory JMM_J
+imports
+  JMM_Framework
+  "../J/Threaded"
+begin
+
+sublocale J_heap_base < red_mthr!: 
+  heap_multithreaded_base 
+    addr2thread_id thread_id2addr
+    empty_heap allocate typeof_addr heap_read heap_write
+    "final_expr" "mred P" convert_RA
+  for P
+.
+
+-- "Move to SmallStep"
+abbreviation J_local_start ::
+  "cname \<Rightarrow> mname \<Rightarrow> ty list \<Rightarrow> ty \<Rightarrow> 'addr J_mb \<Rightarrow> 'addr val list
+  \<Rightarrow> 'addr expr \<times> 'addr locals"
+where
+  "J_local_start \<equiv> 
+  \<lambda>C M Ts T (pns, body) vs. 
+  (blocks (this # pns) (Class C # Ts) (Null # vs) body, empty)"
+
+context J_heap_base begin
+
+abbreviation J_\<E> ::
+  "'addr J_prog \<Rightarrow> cname \<Rightarrow> mname \<Rightarrow> 'addr val list \<Rightarrow> status 
+  \<Rightarrow> ('thread_id \<times> ('addr, 'thread_id) obs_event action) llist set"
+where
+  "J_\<E> P \<equiv> red_mthr.\<E>_start P J_local_start P"
+
+end
+
+end
+
